pico-nosubtyping-limitedvpa/Syntax.v
@@ -116,6 +116,7 @@ Record class_body := {
 Record class_sig := {
   class_qualifier : q_c; (* Mutable, Immutable, or RDM *)
   cname : class_name; (* Class name, need to be the same as the index from class_table *)
+  super : option class_name;
 }.
 
 Record class_def := {
